Some unsuccessful work towards a refine-match syntax

TrieberStack.v
@@ -83,6 +83,32 @@ Next Obligation. (* Guarantee satisfaction! *)
 Qed.
 
 (** *** Pop operation *)
+Require Import RGref.DSL.Fields.
+Inductive nd_fields : Set := val | nxt.
+Instance node_field_type : FieldTyping Node nd_fields.
+Instance nxt_type : FieldType Node nd_fields nxt (option (ref{Node|any}[local_imm,local_imm])) :=
+{ getF := fun x => match x with (mkNode v tl) => tl end;
+  setF := fun x val => match x with (mkNode v tl) => mkNode v val end
+}.
+Check @getF.
+Require Import Utf8.
+Axiom stable_option_match :
+  forall Γ T Γ' A P R G (r:ref{A|P}[R,G]) F f (FT:FieldTyping A F) 
+         (Fx:Set) (FTT:FieldType A F f (option Fx)) Pn Ps,
+         stable Pn R ->
+         (forall (x:Fx), stable (Ps x) R) ->
+         (forall x h, P x h -> @getF _ F FT f _ FTT x = None -> Pn x h) ->
+         (forall x h v, P x h -> getF x = Some v -> Ps v x h) ->
+         (forall (r':ref{A|Pn}[R,G]), r' ≡ r -> rgref Γ T Γ') ->
+         (forall n (r':ref{A|Ps n}[R,G]), r' ≡ r -> rgref Γ T Γ') ->
+         rgref Γ T Γ'.
+(* How do I generalize this a la Mtac? *)
+Notation "'fmatch' r ≫ f 'fwith' | 'None' [[ Pn ]] ==> N | 'Some' x [[ Ps ]] ==> S 'end'" :=
+  (stable_option_match _ _ _ _ _ _ _ r _ f _ _ _ Pn Ps _ _ _ _ 
+                       (fun r' requiv => N)
+                       (fun x r' requiv => S))
+    (at level 44).
+
 Local Obligation Tactic := intros; compute; eauto.
 Program Definition pop_ts {Γ} : ts -> rgref Γ (option nat) Γ :=
   RGFix _ _ (fun rec s =>
@@ -93,6 +119,12 @@ Program Definition pop_ts {Γ} : ts -> rgref Γ (option nat) Γ :=
                        success <- CAS(s,Some hd,tl);
                        if success then rgret (Some n) else rec s
                  end
+                 (*fmatch hd ≫ nxt fwith (* Of course, we don't actually want to match on tl here... *)
+                  | None [[ any ]] ==> rgret None
+                  | Some tl [[ (λ x v h, getF v = Some x) ]] ==> 
+                        (success <- CAS(s,Some hd,tl);
+                         if success then rgret (Some _) else rec s)
+                  end*)
     end).
 Next Obligation.
   f_equal. intros. rewrite H. reflexivity.
